theories/CounterMachines/Reductions/MM2_HALTING_to_CM1_HALT.v
@@ -23,6 +23,8 @@ From Undecidability.CounterMachines.Util Require Import
 
 Require Import ssreflect ssrbool ssrfun.
 
+Set Default Proof Using "Type".
+
 Module Argument.
 Section MM2_CM1.
   Variable (P: list mm2_instr). (* MM2 program *)
