theories/SystemF/Reductions/H10C_SAT_to_SysF_INH.v
@@ -27,6 +27,8 @@ Require Import Undecidability.DiophantineConstraints.H10C.
 
 Require Import ssreflect ssrbool ssrfun.
 
+Set Default Proof Using "Type".
+
 Local Arguments nth_error_In {A l n x}.
 Local Arguments In_nth_error {A l x}.
 Local Arguments Forall_inv {A P a l}.
@@ -942,7 +944,7 @@ Lemma introduce_φ (n: nat):
   ϵ <= S n -> 
   iipc2 (Gamma0 ++ GammaUSP n ++ Gammaφ) (poly_var tt) ->
   iipc2 (Gamma0 ++ GammaUSP n) (poly_var tt).
-Proof.
+Proof using Hφ.
   move: (Hφ). have := δP. rewrite /Gammaφ [Gamma0]lock => + /Forall_forall + Hn.
   elim: (h10cs); first by rewrite app_nil_r.
   move=> [x | x y z | x y z] cs IH /Forall_consP [Hδ /IH {}IH] /Forall_consP /= [Hφc /IH {}IH].
